refactored name-type binding

Hindley-Milner.v
@@ -49,55 +49,19 @@ Module IS := WS.Make(IdDec).
 Module ISF := MSF.WFactsOn(IdDec)(IS).
 Module ISP := MSP.WPropertiesOn(IdDec)(IS).
 
-Section Syntax.
-    Inductive type : Type :=
-        | TUnit
-        | TVar (X : id)
-        | TFun (t1 t2 : type).
+Section TypeMap.
+    Context {T : Type}.
 
-    Inductive expr : Type :=
-        | EUnit
-        | EVar (x : id)
-        | EFun (x : id) (t : type) (e : expr)
-        | EApp (e1 e2 : expr).
+    Definition tmap := id -> option T.
 
-    Definition names : Type := IS.t.
+    Definition tempty : tmap := fun x => None.
 
-    Fixpoint fv (t : type) : names :=
-        match t with
-        | TUnit => IS.empty
-        | TVar X => IS.singleton X
-        | TFun t1 t2 => IS.union (fv t1) (fv t2)
-        end.
-
-    (* type variable in a type *)
-    Fixpoint TIn (X : id) (t : type) : Prop :=
-        match t with
-        | TUnit => False
-        | TVar Y => X = Y
-        | TFun t1 t2 => TIn X t1 \/ TIn X t2
-        end.
-
-    (* type variable in an expression *)
-    Fixpoint EIn (X : id) (e : expr) : Prop :=
-        match e with
-        | EUnit | EVar _ => False
-        | EFun _ t e => TIn X t \/ EIn X e
-        | EApp e1 e2 => EIn X e1 \/ EIn X e2
-        end.
-End Syntax.
-
-Section Gamma.
-    Definition gamma := id -> option type.
-
-    Definition empty : gamma := fun x => None.
-
-    Definition bind (x : id) (t : type) (g : gamma) : gamma :=
-        fun y => if (x =? y)%string then Some t else g y.
+    Definition bind (x : id) (t : T) (m : tmap) : tmap :=
+        fun y => if (x =? y)%string then Some t else m y.
 
     Lemma bind_correct : 
-        forall (x : id) (t : type) (g : gamma),
-        bind x t g x = Some t.
+        forall (x : id) (t : T) (m : tmap),
+        bind x t m x = Some t.
     Proof.
         intros. unfold bind. destruct ((x =? x)%string) eqn:eq.
         - reflexivity.
@@ -105,27 +69,27 @@ Section Gamma.
     Qed. 
 
     Lemma bind_complete :
-        forall (x x' : id) (t t' : type),
+        forall (x x' : id) (t t' : T),
         x' <> x -> 
-        forall (g : gamma),
-        (g x = Some t <-> bind x' t' g x = Some t). 
+        forall (m : tmap),
+        (m x = Some t <-> bind x' t' m x = Some t). 
     Proof.
         intros. unfold bind. apply eqb_neq in H. 
         rewrite H. split; intros; apply H0.
     Qed.
 
     Lemma rebind_correct : 
-        forall (x : id) (t t' : type) (g : gamma),
-        bind x t g = bind x t (bind x t' g).
+        forall (x : id) (t t' : T) (m : tmap),
+        bind x t m = bind x t (bind x t' m).
     Proof.
         intros. apply functional_extensionality. intros y.
         unfold bind. destruct ((x =? y)%string); reflexivity.
     Qed.
 
     Lemma bind_diff_comm : 
-        forall (x y : id) (u v : type) (g : gamma),
+        forall (x y : id) (u v : T) (m : tmap),
         x <> y ->
-        bind x u (bind y v g) = bind y v (bind x u g).
+        bind x u (bind y v m) = bind y v (bind x u m).
     Proof.
         intros. apply functional_extensionality. intros z.
         unfold bind. destruct ((x =? z)%string) eqn:eq.
@@ -135,608 +99,679 @@ Section Gamma.
                 + reflexivity.
             - apply eqb_neq in eq. destruct ((y =? z)%string) eqn:eeq; reflexivity.
     Qed.
-End Gamma.
+End TypeMap.
 
-Section TypeCheck.
-    Inductive check (g : gamma) : expr -> type -> Prop :=
-        | check_unit : 
-            check g EUnit TUnit
-        | check_var : 
-            forall (x : id) (t : type), 
-            g x = Some t ->
-            check g (EVar x) t
-        | check_fun : 
-            forall (x : id) (t1 t2 : type) (e : expr),
-            check (bind x t1 g) e t2 ->
-            check g (EFun x t1 e) (TFun t1 t2)
-        | check_app :
-            forall (e1 e2 : expr) (t1 t2 : type),
-            check g e1 (TFun t1 t2) ->
-            check g e2 t1 ->
-            check g (EApp e1 e2) t2.
-End TypeCheck.
+Module Monomorphic.
+    Section Syntax.
+        Inductive type : Type :=
+            | TUnit
+            | TVar (X : id)
+            | TFun (t1 t2 : type).
 
-Section TypeSubstitution.
-    Definition sigma : Type := id -> option type.
+        Inductive expr : Type :=
+            | EUnit
+            | EVar (x : id)
+            | EFun (x : id) (t : type) (e : expr)
+            | EApp (e1 e2 : expr).
 
-    Definition sempty : sigma := fun _ => None.
+        Definition names : Type := IS.t.
 
-    Definition sbind (X : id) (t : type) (s : sigma) : sigma :=
-        fun Y => if (X =? Y)%string then Some t else s Y.
-
-    Lemma sbind_correct :
-        forall (X : id) (t : type) (s : sigma),
-        sbind X t s X = Some t.
-    Proof.
-        intros X t s. unfold sbind.
-        destruct (X =? X)%string eqn:eq; auto.
-        apply eqb_neq in eq. contradiction.
-    Qed.
-
-    Lemma sbind_complete :
-        forall (X Y : id) (t : type),
-        X <> Y ->
-        forall (s : sigma),
-        sbind X t s Y = s Y.
-    Proof.
-        intros X Y t H s.
-        unfold sbind. apply eqb_neq in H.
-        rewrite H. reflexivity.
-    Qed.
-
-    Fixpoint sub_type (s : sigma) (t : type) : type :=
-        match t with
-        | TUnit => TUnit
-        | TVar X => 
-            match s X with
-            | None => TVar X
-            | Some t' => t'
-            end
-        | TFun t1 t2 => TFun (sub_type s t1) (sub_type s t2)
-        end.
-
-    Lemma sub_type_empty :
-        forall (t : type),
-        sub_type sempty t = t.
-    Proof.
-        intros t. induction t; try reflexivity.
-        simpl. rewrite IHt1. rewrite IHt2.
-        reflexivity.
-    Qed.
-
-    Definition sub_gamma (s : sigma) (g : gamma) : gamma :=
-        fun x =>
-            match g x with
-            | None => None
-            | Some t => Some (sub_type s t)
+        Fixpoint fv (t : type) : names :=
+            match t with
+            | TUnit => IS.empty
+            | TVar X => IS.singleton X
+            | TFun t1 t2 => IS.union (fv t1) (fv t2)
             end.
 
-    (* s2(s1(X)) *)
-    Definition compose_sigma (s1 s2 : sigma) : sigma :=
-        fun X => 
-            match s1 X with
-            | None => s2 X
-            | Some t => Some (sub_type s2 t)
+        (* type variable in a type *)
+        Fixpoint TIn (X : id) (t : type) : Prop :=
+            match t with
+            | TUnit => False
+            | TVar Y => X = Y
+            | TFun t1 t2 => TIn X t1 \/ TIn X t2
             end.
 
-    Lemma compose_empty :
-        forall (s : sigma),
-        s = compose_sigma sempty s.
-    Proof.
-        intros s. apply functional_extensionality.
-        intros x. reflexivity.
-    Qed.
+        (* type variable in an expression *)
+        Fixpoint EIn (X : id) (e : expr) : Prop :=
+            match e with
+            | EUnit | EVar _ => False
+            | EFun _ t e => TIn X t \/ EIn X e
+            | EApp e1 e2 => EIn X e1 \/ EIn X e2
+            end.
+    End Syntax.
 
-    (* Lemma compose_complete :
-        forall (s s' : sigma) (X : id) (t : type),
-        ~ TIn X t ->
-        compose_sigma (sbind X t s) s X = Some t. *)
+    Section TypeCheck.
+        Definition gamma : Type := @tmap type.
 
-    Fixpoint sub_expr (s : sigma) (e : expr) : expr :=
-        match e with
-        | EUnit => EUnit
-        | EVar x => EVar x
-        | EFun x t e => EFun x (sub_type s t) (sub_expr s e)
-        | EApp e1 e2 => EApp (sub_expr s e1) (sub_expr s e2)
-        end.
-    
-    Lemma bind_sub_gamma :
-        forall (s : sigma) (g : gamma) (x : id) (t : type),
-        sub_gamma s (bind x t g) = bind x (sub_type s t) (sub_gamma s g).
-    Proof.
-        intros s g x t. 
-        apply functional_extensionality.
-        intros y. 
-        destruct (IdDec.eq_dec x y); 
-        subst; simpl;
-        unfold sub_gamma;
-        try rewrite bind_correct;
-        try rewrite bind_correct;
-        try reflexivity.
-        unfold bind.
-        apply eqb_neq in n as HF.
-        rewrite HF. reflexivity.
-    Qed.
+        Inductive check (g : gamma) : expr -> type -> Prop :=
+            | check_unit : 
+                check g EUnit TUnit
+            | check_var : 
+                forall (x : id) (t : type), 
+                g x = Some t ->
+                check g (EVar x) t
+            | check_fun : 
+                forall (x : id) (t1 t2 : type) (e : expr),
+                check (bind x t1 g) e t2 ->
+                check g (EFun x t1 e) (TFun t1 t2)
+            | check_app :
+                forall (e1 e2 : expr) (t1 t2 : type),
+                check g e1 (TFun t1 t2) ->
+                check g e2 t1 ->
+                check g (EApp e1 e2) t2.
+    End TypeCheck.
 
-    Theorem substutution_preserves_typing :
-        forall (g : gamma) (e : expr) (t : type),
-        check g e t ->
-        forall (s : sigma),
-        check (sub_gamma s g) (sub_expr s e) (sub_type s t).
-    Proof.
-        intros g e t H. induction H; intros s; try constructor.
-        - unfold sub_gamma. rewrite H. reflexivity.
-        - fold sub_type. fold sub_expr.
-            rewrite <- bind_sub_gamma.
-            apply IHcheck.
-        - apply check_app with (t1 := sub_type s t1);
-            fold sub_expr; auto.
-            specialize IHcheck1 with (s := s).
-            simpl in IHcheck1. assumption.
-    Qed.
+    Section TypeSubstitution.
+        Definition sigma : Type := @tmap type.
 
-    Definition solution (g : gamma) (e : expr) (s : sigma) (t : type) : Prop :=
-    check (sub_gamma s g) (sub_expr s e) t.
-End TypeSubstitution.
+        Fixpoint sub_type (s : sigma) (t : type) : type :=
+            match t with
+            | TUnit => TUnit
+            | TVar X => 
+                match s X with
+                | None => TVar X
+                | Some t' => t'
+                end
+            | TFun t1 t2 => TFun (sub_type s t1) (sub_type s t2)
+            end.
 
-Section ConstraintTyping.
-    Definition equation : Type := type * type.
+        Lemma sub_type_empty :
+            forall (t : type),
+            sub_type tempty t = t.
+        Proof.
+            intros t. induction t; try reflexivity.
+            simpl. rewrite IHt1. rewrite IHt2.
+            reflexivity.
+        Qed.
 
-    Definition constraint : Type := list equation.
-    
-    Definition satisfy_equation (s : sigma) (eq : equation) : Prop :=
-        let (t1,t2) := eq in sub_type s t1 = sub_type s t2.
-    
-    Definition satisfy_constraint (s : sigma) (C : constraint) : Prop :=
-        Forall (satisfy_equation s) C.
+        Definition sub_gamma (s : sigma) (g : gamma) : gamma :=
+            fun x =>
+                match g x with
+                | None => None
+                | Some t => Some (sub_type s t)
+                end.
 
-    (* type variable in an equation *)
-    Fixpoint EQIn (X : id) (eq : equation) : Prop :=
-        let (t1,t2) := eq in TIn X t1 \/ TIn X t2.
+        (* s2(s1(X)) *)
+        Definition compose_sigma (s1 s2 : sigma) : sigma :=
+            fun X => 
+                match s1 X with
+                | None => s2 X
+                | Some t => Some (sub_type s2 t)
+                end.
 
-    (* type variable in a constraint *)
-    Definition CIn (X : id) (C : constraint) : Prop :=
-        Exists (EQIn X) C.
+        Lemma compose_empty :
+            forall (s : sigma),
+            s = compose_sigma tempty s.
+        Proof.
+            intros s. apply functional_extensionality.
+            intros x. reflexivity.
+        Qed.
 
-    (* type variable not in gamma *)
-    Definition GNIn (X : id) (g : gamma) : Prop :=
-        forall (x : id) (t : type),
-        g x = Some t -> ~ TIn X t.
+        Fixpoint sub_expr (s : sigma) (e : expr) : expr :=
+            match e with
+            | EUnit => EUnit
+            | EVar x => EVar x
+            | EFun x t e => EFun x (sub_type s t) (sub_expr s e)
+            | EApp e1 e2 => EApp (sub_expr s e1) (sub_expr s e2)
+            end.
+        
+        Lemma bind_sub_gamma :
+            forall (s : sigma) (g : gamma) (x : id) (t : type),
+            sub_gamma s (bind x t g) = bind x (sub_type s t) (sub_gamma s g).
+        Proof.
+            intros s g x t. 
+            apply functional_extensionality.
+            intros y. 
+            destruct (IdDec.eq_dec x y); 
+            subst; simpl;
+            unfold sub_gamma;
+            try rewrite bind_correct;
+            try rewrite bind_correct;
+            try reflexivity.
+            unfold bind.
+            apply eqb_neq in n as HF.
+            rewrite HF. reflexivity.
+        Qed.
 
-    Inductive constraint_type (g : gamma) 
-    : expr -> type -> names -> constraint -> Prop :=
-        | ct_unit : 
-            constraint_type g EUnit TUnit IS.empty []
-        | ct_var :
+        Theorem substutution_preserves_typing :
+            forall (g : gamma) (e : expr) (t : type),
+            check g e t ->
+            forall (s : sigma),
+            check (sub_gamma s g) (sub_expr s e) (sub_type s t).
+        Proof.
+            intros g e t H. induction H; intros s; try constructor.
+            - unfold sub_gamma. rewrite H. reflexivity.
+            - fold sub_type. fold sub_expr.
+                rewrite <- bind_sub_gamma.
+                apply IHcheck.
+            - apply check_app with (t1 := sub_type s t1);
+                fold sub_expr; auto.
+                specialize IHcheck1 with (s := s).
+                simpl in IHcheck1. assumption.
+        Qed.
+
+        Definition solution (g : gamma) (e : expr) (s : sigma) (t : type) : Prop :=
+        check (sub_gamma s g) (sub_expr s e) t.
+    End TypeSubstitution.
+
+    Section ConstraintTyping.
+        Definition equation : Type := type * type.
+
+        Definition constraint : Type := list equation.
+        
+        Definition satisfy_equation (s : sigma) (eq : equation) : Prop :=
+            let (t1,t2) := eq in sub_type s t1 = sub_type s t2.
+        
+        Definition satisfy_constraint (s : sigma) (C : constraint) : Prop :=
+            Forall (satisfy_equation s) C.
+
+        (* type variable in an equation *)
+        Fixpoint EQIn (X : id) (eq : equation) : Prop :=
+            let (t1,t2) := eq in TIn X t1 \/ TIn X t2.
+
+        (* type variable in a constraint *)
+        Definition CIn (X : id) (C : constraint) : Prop :=
+            Exists (EQIn X) C.
+
+        (* type variable not in gamma *)
+        Definition GNIn (X : id) (g : gamma) : Prop :=
             forall (x : id) (t : type),
-            g x = Some t ->
-            constraint_type g (EVar x) t IS.empty []
-        | ct_fun :
-            forall (x : id) (t1 t2 : type) 
-                (e : expr) (X : names) (C : constraint),
-            constraint_type (bind x t1 g) e t2 X C ->
-            constraint_type g (EFun x t1 e) (TFun t1 t2) X C
-        | ct_app :
-            forall (e1 e2 : expr) (t1 t2 : type) (X : id)
-                (X1 X2 : names) (C1 C2 : constraint),
-            constraint_type g e1 t1 X1 C1 ->
-            constraint_type g e2 t2 X2 C2 ->
-            IS.Empty (IS.inter X1 X2) ->
-            IS.Empty (IS.inter X1 (fv t2)) ->
-            IS.Empty (IS.inter X2 (fv t1)) ->
-            ~ IS.In X X1 -> ~ IS.In X X2 ->
-            ~ TIn X t1 -> ~ TIn X t2 ->
-            ~ EIn X e1 -> ~ EIn X e2 ->
-            ~ CIn X C1 -> ~ CIn X C2 -> GNIn X g ->
-            constraint_type g (EApp e1 e2) (TVar X)
-                (IS.add X (IS.union X1 X2))
-                ((t1, TFun t2 (TVar X)) :: C1 ++ C2).
+            g x = Some t -> ~ TIn X t.
 
-    (* standard library lemma *)
-    Axiom Forall_app : 
-        forall {A : Type} (P : A -> Prop) (l1 l2 : list A),
-    Forall P (l1 ++ l2) <-> Forall P l1 /\ Forall P l2.
+        Inductive constraint_type (g : gamma) 
+        : expr -> type -> names -> constraint -> Prop :=
+            | ct_unit : 
+                constraint_type g EUnit TUnit IS.empty []
+            | ct_var :
+                forall (x : id) (t : type),
+                g x = Some t ->
+                constraint_type g (EVar x) t IS.empty []
+            | ct_fun :
+                forall (x : id) (t1 t2 : type) 
+                    (e : expr) (X : names) (C : constraint),
+                constraint_type (bind x t1 g) e t2 X C ->
+                constraint_type g (EFun x t1 e) (TFun t1 t2) X C
+            | ct_app :
+                forall (e1 e2 : expr) (t1 t2 : type) (X : id)
+                    (X1 X2 : names) (C1 C2 : constraint),
+                constraint_type g e1 t1 X1 C1 ->
+                constraint_type g e2 t2 X2 C2 ->
+                IS.Empty (IS.inter X1 X2) ->
+                IS.Empty (IS.inter X1 (fv t2)) ->
+                IS.Empty (IS.inter X2 (fv t1)) ->
+                ~ IS.In X X1 -> ~ IS.In X X2 ->
+                ~ TIn X t1 -> ~ TIn X t2 ->
+                ~ EIn X e1 -> ~ EIn X e2 ->
+                ~ CIn X C1 -> ~ CIn X C2 -> GNIn X g ->
+                constraint_type g (EApp e1 e2) (TVar X)
+                    (IS.add X (IS.union X1 X2))
+                    ((t1, TFun t2 (TVar X)) :: C1 ++ C2).
 
-    Definition constraint_solution 
-    {g : gamma} {e : expr} {t : type} {X : names} {C : constraint}
-    (H : constraint_type g e t X C) (s : sigma) (T : type) : Prop :=
-    satisfy_constraint s C /\ sub_type s t = T.
+        (* standard library lemma *)
+        Axiom Forall_app : 
+            forall {A : Type} (P : A -> Prop) (l1 l2 : list A),
+        Forall P (l1 ++ l2) <-> Forall P l1 /\ Forall P l2.
 
-    Theorem Constraint_Typing_Sound : 
-        forall (g : gamma) (e : expr) (t : type) 
+        Definition constraint_solution 
+        {g : gamma} {e : expr} {t : type} {X : names} {C : constraint}
+        (H : constraint_type g e t X C) (s : sigma) (T : type) : Prop :=
+        satisfy_constraint s C /\ sub_type s t = T.
+
+        Theorem Constraint_Typing_Sound : 
+            forall (g : gamma) (e : expr) (t : type) 
+                (X : names) (C : constraint) 
+                (H : constraint_type g e t X C) 
+                (s : sigma) (T : type),
+            constraint_solution H s T -> solution g e s T.
+        Proof.
+            intros g e t X C H s T HCS.
+            destruct HCS as [HSC HSE].
+            unfold solution. subst.
+            induction H.
+            - constructor.
+            - apply substutution_preserves_typing.
+                constructor; auto.
+            - constructor.
+                fold sub_type. fold sub_expr.
+                rewrite <- bind_sub_gamma. auto.
+            - inv HSC.
+                apply Forall_app in H16 as [HC1 HC2].
+                apply check_app with (t1 := sub_type s t2); auto.
+                fold sub_expr.
+                apply IHconstraint_type1 in HC1.
+                unfold satisfy_equation in H15.
+                rewrite H15 in HC1. simpl in HC1.
+                assumption.
+        Qed.
+
+        (* s/N *)
+        Definition sigma_diff (s : sigma) (N : names) : sigma := 
+            fun X => if IS.mem X N then None else s X.
+
+        Theorem Constraint_Typing_Complete : 
+            forall (g : gamma) (e : expr) (t : type) 
             (X : names) (C : constraint) 
             (H : constraint_type g e t X C) 
             (s : sigma) (T : type),
-        constraint_solution H s T -> solution g e s T.
-    Proof.
-        intros g e t X C H s T HCS.
-        destruct HCS as [HSC HSE].
-        unfold solution. subst.
-        induction H.
-        - constructor.
-        - apply substutution_preserves_typing.
-            constructor; auto.
-        - constructor.
-            fold sub_type. fold sub_expr.
-            rewrite <- bind_sub_gamma. auto.
-        - inv HSC.
-            apply Forall_app in H16 as [HC1 HC2].
-            apply check_app with (t1 := sub_type s t2); auto.
-            fold sub_expr.
-            apply IHconstraint_type1 in HC1.
-            unfold satisfy_equation in H15.
-            rewrite H15 in HC1. simpl in HC1.
-            assumption.
-    Qed.
+            sigma_diff s X = s ->
+            solution g e s T ->
+            exists (s' : sigma),
+            sigma_diff s' X = s /\ constraint_solution H s' T.
+        Proof.
+            intros g e t X C H.
+            (* Coq won't let me do induction on H *)
+            (* induction H. *)
+        Abort.
+    End ConstraintTyping.
 
-    (* s/N *)
-    Definition sigma_diff (s : sigma) (N : names) : sigma := 
-        fun X => if IS.mem X N then None else s X.
+    Section Unification.
+        Definition sub_equation (s : sigma) (eq : equation) : equation :=
+            let (t1,t2) := eq in (sub_type s t1, sub_type s t2).
 
-    Theorem Constraint_Typing_Complete : 
-        forall (g : gamma) (e : expr) (t : type) 
-        (X : names) (C : constraint) 
-        (H : constraint_type g e t X C) 
-        (s : sigma) (T : type),
-        sigma_diff s X = s ->
-        solution g e s T ->
-        exists (s' : sigma),
-        sigma_diff s' X = s /\ constraint_solution H s' T.
-    Proof.
-        intros g e t X C H.
-        (* Coq won't let me do induction on H *)
-        (* induction H. *)
-    Abort.
-End ConstraintTyping.
+        Definition sub_constraint (s : sigma) (C : constraint) : constraint :=
+            map (sub_equation s) C.
 
-Section Unification.
-    Definition sub_equation (s : sigma) (eq : equation) : equation :=
-        let (t1,t2) := eq in (sub_type s t1, sub_type s t2).
+        Inductive unify : constraint -> sigma -> Prop :=
+            | unify_nil : unify [] tempty
+            | unify_eq : 
+                forall (t : type) (C : constraint) (s : sigma),
+                unify C s ->
+                unify ((t,t) :: C) s
+            | unify_left_var :
+                forall (X : id) (t : type) (C : constraint) (s : sigma),
+                ~ TIn X t ->
+                unify (sub_constraint (bind X t tempty) C) s ->
+                unify ((TVar X, t) :: C) (compose_sigma (bind X t tempty) s)
+            | unify_right_var :
+                forall (X : id) (t : type) (C : constraint) (s : sigma),
+                ~ TIn X t ->
+                unify (sub_constraint (bind X t tempty) C) s ->
+                unify ((t, TVar X) :: C) (compose_sigma (bind X t tempty) s)
+            | unify_fun : 
+                forall (a1 a2 b1 b2 : type) (C : constraint) (s : sigma),
+                unify ((a1,a2) :: (b1,b2) :: C) s ->
+                unify ((TFun a1 b1, TFun a2 b2) :: C) s.
 
-    Definition sub_constraint (s : sigma) (C : constraint) : constraint :=
-        map (sub_equation s) C.
+        Definition more_general (s s' : sigma) : Prop :=
+            exists (s'' : sigma), s' = compose_sigma s s''.
 
-    Inductive unify : constraint -> sigma -> Prop :=
-        | unify_nil : unify [] sempty
-        | unify_eq : 
-            forall (t : type) (C : constraint) (s : sigma),
-            unify C s ->
-            unify ((t,t) :: C) s
-        | unify_left_var :
-            forall (X : id) (t : type) (C : constraint) (s : sigma),
+        Definition principal_unifier (C : constraint) (s : sigma) : Prop := 
+            satisfy_constraint s C /\ 
+            forall (s' : sigma), 
+            satisfy_constraint s' C ->  more_general s s'.
+        
+        Lemma satisfy_equation_compose :
+            forall (X : id) (t : type) (s : sigma),
             ~ TIn X t ->
-            unify (sub_constraint (sbind X t sempty) C) s ->
-            unify ((TVar X, t) :: C) (compose_sigma (sbind X t sempty) s)
-        | unify_right_var :
-            forall (X : id) (t : type) (C : constraint) (s : sigma),
-            ~ TIn X t ->
-            unify (sub_constraint (sbind X t sempty) C) s ->
-            unify ((t, TVar X) :: C) (compose_sigma (sbind X t sempty) s)
-        | unify_fun : 
-            forall (a1 a2 b1 b2 : type) (C : constraint) (s : sigma),
-            unify ((a1,a2) :: (b1,b2) :: C) s ->
-            unify ((TFun a1 b1, TFun a2 b2) :: C) s.
-
-    Definition more_general (s s' : sigma) : Prop :=
-        exists (s'' : sigma), s' = compose_sigma s s''.
-
-    Definition principal_unifier (C : constraint) (s : sigma) : Prop := 
-        satisfy_constraint s C /\ 
-        forall (s' : sigma), 
-        satisfy_constraint s' C ->  more_general s s'.
-    
-    Lemma satisfy_equation_compose :
-        forall (X : id) (t : type) (s : sigma),
-        ~ TIn X t ->
-        satisfy_equation (compose_sigma (sbind X t sempty) s) (TVar X, t).
-    Proof.
-        intros X t s H.
-        unfold satisfy_equation.
-        unfold compose_sigma. simpl.
-        rewrite sbind_correct.
-        (* Intuitively true. *)
-        (* generalize dependent X. *)
-        (* generalize dependent s. *)
-        induction t; 
-        (* intros s X H;  *)
-        auto.
-        - assert (HXX : X <> X0).
-            + intros HF. apply H. subst.
-                reflexivity.
-            + simpl. rewrite (sbind_complete X X0 
-                (TVar X0) HXX). unfold sempty.
-                reflexivity.
-        - simpl in H. 
-            apply CP.not_or_and in H as [H1 H2].
-            apply IHt1 in H1. apply IHt2 in H2.
-            simpl. rewrite H1. rewrite H2.
-            (* This case makes no sense. *)
-    Admitted.
-
-    Lemma satisfy_equation_sym :
-        forall (s : sigma) (t1 t2 : type),
-        satisfy_equation s (t1,t2) ->
-        satisfy_equation s (t2,t1).
-    Proof.
-        intros s t1 t2 H. 
-        unfold satisfy_equation in *. auto.
-    Qed.
-
-    Lemma satisfy_constraint_compose :
-        forall (s : sigma) (X : id) (t : type) (C : constraint),
-        satisfy_constraint s (sub_constraint (sbind X t sempty) C) ->
-        satisfy_constraint (compose_sigma (sbind X t sempty) s) C.
-    Proof.
-        intros s X t C H.
-        unfold satisfy_constraint in *.
-        induction C; constructor; inv H; auto.
-        destruct a as [t1 t2].
-        unfold satisfy_equation in *.
-        simpl in H2. clear H3 IHC H.
-        unfold compose_sigma.
-        destruct t1; destruct t2;
-        simpl in *; auto;
-        try destruct (sbind X t sempty X0); 
-        try destruct (sbind X t sempty X1);
-        auto; try discriminate.
-    Admitted.
-
-    Theorem unify_correct :
-        forall (C : constraint) (s : sigma),
-        unify C s -> principal_unifier C s.
-    Proof.
-        intros C s HU. unfold principal_unifier.
-        induction HU; split;
-        try (intros s' HSC; unfold more_general).
-        - constructor.
-        - exists s'. apply compose_empty.
-        - destruct IHHU as [HS _].
-            constructor; auto.
+            satisfy_equation (compose_sigma (bind X t tempty) s) (TVar X, t).
+        Proof.
+            intros X t s H.
             unfold satisfy_equation.
-            reflexivity.
-        - inv HSC. destruct IHHU as [_ IH].
-            apply IH in H2. assumption.
-        - destruct IHHU as [IH _].
-            constructor.
-            + apply satisfy_equation_compose. assumption.
-            + apply satisfy_constraint_compose. assumption.
-        - inv HSC. destruct IHHU as [_ IH]. admit.
-        - destruct IHHU as [IH _].
-            constructor.
-            + apply satisfy_equation_sym.
-                apply satisfy_equation_compose.
-                assumption.
-            + apply satisfy_constraint_compose. assumption.
-        - admit.
-        - destruct IHHU as [IH _]. inv IH.
-            inv H2. constructor; auto.
+            unfold compose_sigma. simpl.
+            rewrite bind_correct.
+            (* Intuitively true. *)
+            (* generalize dependent X. *)
+            (* generalize dependent s. *)
+            induction t; 
+            (* intros s X H;  *)
+            auto.
+            - assert (HXX : X <> X0).
+                + intros HF. apply H. subst.
+                    reflexivity.
+                + simpl. admit.
+            - simpl in H. 
+                apply CP.not_or_and in H as [H1 H2].
+                apply IHt1 in H1. apply IHt2 in H2.
+                simpl. rewrite H1. rewrite H2.
+                (* This case makes no sense. *)
+        Admitted.
+
+        Lemma satisfy_equation_sym :
+            forall (s : sigma) (t1 t2 : type),
+            satisfy_equation s (t1,t2) ->
+            satisfy_equation s (t2,t1).
+        Proof.
+            intros s t1 t2 H. 
+            unfold satisfy_equation in *. auto.
+        Qed.
+
+        Lemma satisfy_constraint_compose :
+            forall (s : sigma) (X : id) (t : type) (C : constraint),
+            satisfy_constraint s (sub_constraint (bind X t tempty) C) ->
+            satisfy_constraint (compose_sigma (bind X t tempty) s) C.
+        Proof.
+            intros s X t C H.
+            unfold satisfy_constraint in *.
+            induction C; constructor; inv H; auto.
+            destruct a as [t1 t2].
             unfold satisfy_equation in *.
-            clear H2 H4. simpl.
-            rewrite H1. rewrite H3.
-            reflexivity.
-        - destruct IHHU as [_ IH].
-            assert (H : satisfy_constraint 
-                s' ((a1, a2) :: (b1, b2) :: C)).
-            + inv HSC. inv H1.
+            simpl in H2. clear H3 IHC H.
+            unfold compose_sigma.
+            destruct t1; destruct t2;
+            simpl in *; auto;
+            try destruct (sbind X t sempty X0); 
+            try destruct (sbind X t sempty X1);
+            auto; try discriminate.
+        Admitted.
+
+        Theorem unify_correct :
+            forall (C : constraint) (s : sigma),
+            unify C s -> principal_unifier C s.
+        Proof.
+            intros C s HU. unfold principal_unifier.
+            induction HU; split;
+            try (intros s' HSC; unfold more_general).
+            - constructor.
+            - exists s'. apply compose_empty.
+            - destruct IHHU as [HS _].
                 constructor; auto.
-            + apply IH in H. assumption.
-    Admitted.    
-End Unification.
+                unfold satisfy_equation.
+                reflexivity.
+            - inv HSC. destruct IHHU as [_ IH].
+                apply IH in H2. assumption.
+            - destruct IHHU as [IH _].
+                constructor.
+                + apply satisfy_equation_compose. assumption.
+                + apply satisfy_constraint_compose. assumption.
+            - inv HSC. destruct IHHU as [_ IH]. admit.
+            - destruct IHHU as [IH _].
+                constructor.
+                + apply satisfy_equation_sym.
+                    apply satisfy_equation_compose.
+                    assumption.
+                + apply satisfy_constraint_compose. assumption.
+            - admit.
+            - destruct IHHU as [IH _]. inv IH.
+                inv H2. constructor; auto.
+                unfold satisfy_equation in *.
+                clear H2 H4. simpl.
+                rewrite H1. rewrite H3.
+                reflexivity.
+            - destruct IHHU as [_ IH].
+                assert (H : satisfy_constraint 
+                    s' ((a1, a2) :: (b1, b2) :: C)).
+                + inv HSC. inv H1.
+                    constructor; auto.
+                + apply IH in H. assumption.
+        Admitted.
+    End Unification.
 
-Section PrincipalTypes.
-    Definition principal_solution
-    {g : gamma} {e : expr} {t : type} {X : names} {C : constraint}
-    (H : constraint_type g e t X C) (s : sigma) (T : type) : Prop :=
-    constraint_solution H s T /\
-    forall (s' : sigma) (T' : type),
-    constraint_solution H s' T' -> more_general s s'.
+    Section PrincipalTypes.
+        Definition principal_solution
+        {g : gamma} {e : expr} {t : type} {X : names} {C : constraint}
+        (H : constraint_type g e t X C) (s : sigma) (T : type) : Prop :=
+        constraint_solution H s T /\
+        forall (s' : sigma) (T' : type),
+        constraint_solution H s' T' -> more_general s s'.
 
-    Corollary unify_principal_solution :
-        forall {g : gamma} {e : expr} {t : type} {X : names} {C : constraint}
-            (H : constraint_type g e t X C) (s : sigma),
-        unify C s ->
-        principal_solution H s (sub_type s t).
-    Proof.
-        intros g e t X C H s HU.
-        apply unify_correct in HU as HUC.
-        unfold principal_unifier in HUC.
-        unfold principal_solution.
-        destruct HUC as [HSC HMG]. split.
-        - unfold constraint_solution. split; auto.
-        - intros s' T' Hs'T'.
-            unfold constraint_solution in Hs'T'.
-            destruct Hs'T' as [HSCs' HSTs']. auto.
-    Qed.
+        Corollary unify_principal_solution :
+            forall {g : gamma} {e : expr} {t : type} {X : names} {C : constraint}
+                (H : constraint_type g e t X C) (s : sigma),
+            unify C s ->
+            principal_solution H s (sub_type s t).
+        Proof.
+            intros g e t X C H s HU.
+            apply unify_correct in HU as HUC.
+            unfold principal_unifier in HUC.
+            unfold principal_solution.
+            destruct HUC as [HSC HMG]. split.
+            - unfold constraint_solution. split; auto.
+            - intros s' T' Hs'T'.
+                unfold constraint_solution in Hs'T'.
+                destruct Hs'T' as [HSCs' HSTs']. auto.
+        Qed.
 
-    Lemma constraint_solution_unify :
-        forall {g : gamma} {e : expr} {t : type} {X : names} {C : constraint}
-            (H : constraint_type g e t X C) (s' : sigma) (T' : type),
-        constraint_solution H s' T' ->
-        exists (s : sigma), unify C s.
-    Proof.
-        intros g e t X C H s' T' HCS.
-        unfold constraint_solution in HCS.
-        destruct HCS as [HSC HST].
-        dependent induction H; simpl in *;
-        try (exists sempty; apply unify_nil).
-        - apply IHconstraint_type
-            with (T' := sub_type s' t2) in HSC; auto.
-        - inv HSC. apply Forall_app in H16 as [HC1 HC2].
-            apply IHconstraint_type1 
-                with (T' := sub_type s' t1) in HC1; auto.
-            apply IHconstraint_type2
-                with (T' := sub_type s' t2) in HC2; auto.
-            destruct HC1 as [s1 HU1].
-            destruct HC2 as [s2 HU2].
-            destruct t1.
-            + inv H15.
-            + exists (compose_sigma (sbind X0 (TFun t2 (TVar X)) sempty) (compose_sigma s1 s2)).
-                constructor; admit.
-            + exists (compose_sigma s1 s2).
-                constructor. admit.
-    Admitted.
-
-    Theorem principal_types :
-        forall {g : gamma} {e : expr} {t : type} {X : names} {C : constraint}
-            (H : constraint_type g e t X C),
-        (exists (s' : sigma) (T' : type), constraint_solution H s' T') ->
-        exists (s : sigma) (T : type), principal_solution H s T.
-    Proof.
-        intros g e t X C H [s' [T' HCS]].
-        apply constraint_solution_unify in HCS.
-        destruct HCS as [s HU].
-        exists s. exists (sub_type s t).
-        apply unify_principal_solution; auto.
-    Qed.
-
-    (* Interleave constraint generation and unification. 
-        Should generate a principal type at each step. *)
-    Inductive interleave (g : gamma) : expr -> type -> Prop :=
-        | il_unit : interleave g EUnit TUnit
-        | il_var : 
-            forall (x : id) (t : type),
-            g x = Some t ->
-            interleave g (EVar x) t
-        | il_fun :
-            forall (x : id) (t1 t2 : type) (e : expr),
-            interleave (bind x t1 g) e t2 ->
-            interleave g (EFun x t1 e) (TFun t1 t2)
-        | il_app :
-            forall (e1 e2 : expr) (t1 t2 : type) (X : id) (s : sigma),
-            interleave g e1 t1 ->
-            interleave g e2 t2 ->
-            ~ TIn X t1 -> ~ TIn X t2 ->
-            ~ EIn X e1 -> ~ EIn X e2 -> GNIn X g ->
-            unify [(t1, TFun t2 (TVar X))] s ->
-            interleave g (EApp e1 e2) (sub_type s (TVar X)).
-
-    Proposition interleave_sound :
-        forall (g : gamma) (e : expr) (t : type),
-        interleave g e t ->
-        forall (N : names) (C : constraint)
-            (H : constraint_type g e t N C),
-        exists (s : sigma), unify C s /\ constraint_solution H s t.
-    Proof.
-        intros g e t HIL. 
-        induction HIL; intros N C HCT; inv HCT;
-        unfold constraint_solution.
-        - exists sempty. repeat split; constructor.
-        - exists sempty. repeat split; 
-            try constructor. apply sub_type_empty.
-        - pose proof IHHIL N C H5 as IH.
-            destruct IH as [s [HU HCS]].
+        Lemma constraint_solution_unify :
+            forall {g : gamma} {e : expr} {t : type} {X : names} {C : constraint}
+                (H : constraint_type g e t X C) (s' : sigma) (T' : type),
+            constraint_solution H s' T' ->
+            exists (s : sigma), unify C s.
+        Proof.
+            intros g e t X C H s' T' HCS.
             unfold constraint_solution in HCS.
-            exists s. destruct HCS as [HSC HST].
-            repeat split; auto.
-            simpl. rewrite HST. admit.
-        - admit.
-        (* white flag. *)
-        (* pose proof IHHIL1 X1 C1 H8 as IH1. *)
-    Abort.
-End PrincipalTypes.
+            destruct HCS as [HSC HST].
+            dependent induction H; simpl in *;
+            try (exists tempty; apply unify_nil).
+            - apply IHconstraint_type
+                with (T' := sub_type s' t2) in HSC; auto.
+            - inv HSC. apply Forall_app in H16 as [HC1 HC2].
+                apply IHconstraint_type1 
+                    with (T' := sub_type s' t1) in HC1; auto.
+                apply IHconstraint_type2
+                    with (T' := sub_type s' t2) in HC2; auto.
+                destruct HC1 as [s1 HU1].
+                destruct HC2 as [s2 HU2].
+                destruct t1.
+                + inv H15.
+                + exists (compose_sigma (bind X0 (TFun t2 (TVar X)) tempty) (compose_sigma s1 s2)).
+                    constructor; admit.
+                + exists (compose_sigma s1 s2).
+                    constructor. admit.
+        Admitted.
 
-(* Definition scheme : Type := list id * type.
+        Theorem principal_types :
+            forall {g : gamma} {e : expr} {t : type} {X : names} {C : constraint}
+                (H : constraint_type g e t X C),
+            (exists (s' : sigma) (T' : type), constraint_solution H s' T') ->
+            exists (s : sigma) (T : type), principal_solution H s T.
+        Proof.
+            intros g e t X C H [s' [T' HCS]].
+            apply constraint_solution_unify in HCS.
+            destruct HCS as [s HU].
+            exists s. exists (sub_type s t).
+            apply unify_principal_solution; auto.
+        Qed.
 
-Definition void : scheme := (["X"],TVar "X"). *)
+        (* Interleave constraint generation and unification. 
+            Should generate a principal type at each step. *)
+        Inductive interleave (g : gamma) : expr -> type -> Prop :=
+            | il_unit : interleave g EUnit TUnit
+            | il_var : 
+                forall (x : id) (t : type),
+                g x = Some t ->
+                interleave g (EVar x) t
+            | il_fun :
+                forall (x : id) (t1 t2 : type) (e : expr),
+                interleave (bind x t1 g) e t2 ->
+                interleave g (EFun x t1 e) (TFun t1 t2)
+            | il_app :
+                forall (e1 e2 : expr) (t1 t2 : type) (X : id) (s : sigma),
+                interleave g e1 t1 ->
+                interleave g e2 t2 ->
+                ~ TIn X t1 -> ~ TIn X t2 ->
+                ~ EIn X e1 -> ~ EIn X e2 -> GNIn X g ->
+                unify [(t1, TFun t2 (TVar X))] s ->
+                interleave g (EApp e1 e2) (sub_type s (TVar X)).
 
-Inductive poly : Type :=
-    | PType (t : type)
-    | PForall (X : id) (t : poly).
+        Proposition interleave_sound :
+            forall (g : gamma) (e : expr) (t : type),
+            interleave g e t ->
+            forall (N : names) (C : constraint)
+                (H : constraint_type g e t N C),
+            exists (s : sigma), unify C s /\ constraint_solution H s t.
+        Proof.
+            intros g e t HIL. 
+            induction HIL; intros N C HCT; inv HCT;
+            unfold constraint_solution.
+            - exists tempty. repeat split; constructor.
+            - exists tempty. repeat split; 
+                try constructor. apply sub_type_empty.
+            - pose proof IHHIL N C H5 as IH.
+                destruct IH as [s [HU HCS]].
+                unfold constraint_solution in HCS.
+                exists s. destruct HCS as [HSC HST].
+                repeat split; auto.
+                simpl. rewrite HST. admit.
+            - admit.
+            (* white flag. *)
+            (* pose proof IHHIL1 X1 C1 H8 as IH1. *)
+        Abort.
+    End PrincipalTypes.
 
-Section Examples.
-    Ltac ex222 t :=
-        apply check_app with (t1 := t);
-        constructor; reflexivity.
-
-    Definition f : id := "f".
-    Definition a : id := "a".
-    Definition x : id := "x".
-    Definition y : id := "y".
-    Definition z : id := "z".
-    Definition X : id := "X".
-    Definition Y : id := "Y".
-    Definition Z : id := "Z".
-    
-    Definition g : gamma := bind f (TVar X) (bind a (TVar Y) empty).
-    Definition e : expr := EApp (EVar f) (EVar a).
-    
-    Example ex2221 : 
-        solution g e (sbind X (TFun (TVar Y) TUnit) sempty) TUnit.
-    Proof. ex222 (TVar Y). Qed.
-
-    Example ex2222 :
-        solution g e (sbind X (TFun (TVar Y) (TVar Z)) (sbind Z TUnit sempty)) (TVar Z).
-    Proof. ex222 (TVar Y). Qed.
-
-    Example ex2223 :
-        solution g e (sbind X (TFun TUnit TUnit) (sbind Y TUnit sempty)) TUnit.
-    Proof. ex222 TUnit. Qed.
-
-    Example ex224 :
-        solution g e (sbind X (TFun (TVar Y) (TVar Z)) sempty) (TVar Z).
-    Proof. ex222 (TVar Y). Qed.
-    
-    Example ex2225 :
-        solution g e (sbind X (TFun (TVar Y) (TFun TUnit TUnit)) sempty) (TFun TUnit TUnit).
-    Proof. ex222 (TVar Y). Qed.
-
-    Definition term : expr := 
-        EFun x (TVar X) (EFun y (TVar Y) (EFun z (TVar Z) 
-            (EApp (EApp (EVar x) (EVar z)) (EApp (EVar y) (EVar z))))).
-
-    Example ex2231 : 
-        let s := (sbind Y (TFun (TVar Z) TUnit) (sbind X (TFun (TVar Z) (TFun TUnit TUnit)) sempty)) in
-        solution empty term s (sub_type s (TFun (TVar X) (TFun (TVar Y) (TFun (TVar Z) TUnit)))).
-    Proof.
-        unfold solution. simpl.
-        repeat apply check_fun.
-        apply check_app with (t1 := TUnit).
-        - apply check_app with (t1 := TVar Z);
+    Section Examples.
+        Ltac ex222 t :=
+            apply check_app with (t1 := t);
             constructor; reflexivity.
-        - apply check_app with (t1 := TVar Z);
-            constructor; reflexivity.
-    Qed.
 
-    Ltac ct_app_apply :=
-        apply ct_app; 
-        try (intros HF; simpl in HF;
-            subst; discriminate);
-        try (intros HF; simpl in HF;
-            subst; contradiction).
+        Definition f : id := "f".
+        Definition a : id := "a".
+        Definition x : id := "x".
+        Definition y : id := "y".
+        Definition z : id := "z".
+        Definition X : id := "X".
+        Definition Y : id := "Y".
+        Definition Z : id := "Z".
+        
+        Definition g : gamma := bind f (TVar X) (bind a (TVar Y) tempty).
+        Definition e : expr := EApp (EVar f) (EVar a).
+        
+        Example ex2221 : 
+            solution g e (bind X (TFun (TVar Y) TUnit) tempty) TUnit.
+        Proof. ex222 (TVar Y). Qed.
 
-    (* MSet library is a pain to work with... *)
-    Axiom empty_inter :
-        forall (x y : id),
-        x <> y <-> 
-        IS.Empty (IS.inter (IS.singleton x) (IS.singleton y)).
+        Example ex2222 :
+            solution g e (bind X (TFun (TVar Y) (TVar Z)) (bind Z TUnit tempty)) (TVar Z).
+        Proof. ex222 (TVar Y). Qed.
 
-    Example ex2233 :
-        exists (t : type) (N : names) (C : constraint),
-        constraint_type empty term t N C.
-    Proof.
-        unfold term.
-        remember "T" as T in *.
-        remember "U" as U in *.
-        remember "V" as V in *.
-        remember "W" as W in *.
-        exists (TFun (TVar X) (TFun (TVar Y) (TFun (TVar Z) (TVar W)))).
-        exists (IS.add W 
-            (IS.union 
-                (IS.add U (IS.union IS.empty IS.empty))
-                (IS.add V (IS.union IS.empty IS.empty)))).
-        exists ((TVar U, TFun (TVar V) (TVar W)) :: 
-            ((TVar X, TFun (TVar Z) (TVar U)) :: [] ++ []) ++
-            ((TVar Y, TFun (TVar Z) (TVar V)) :: [] ++ [])).
-        repeat apply ct_fun.
-        ct_app_apply.
-        - ct_app_apply;
-            try (constructor; reflexivity);
-            try apply ISP.empty_inter_1;
-            try apply ISP.empty_inter_2;
-            try apply IS.empty_spec.
-            + intros HF; inv HF.
-            + intros HF; inv HF.
-            + intros q Q Hq HIn.
+        Example ex2223 :
+            solution g e (bind X (TFun TUnit TUnit) (bind Y TUnit tempty)) TUnit.
+        Proof. ex222 TUnit. Qed.
+
+        Example ex224 :
+            solution g e (bind X (TFun (TVar Y) (TVar Z)) tempty) (TVar Z).
+        Proof. ex222 (TVar Y). Qed.
+        
+        Example ex2225 :
+            solution g e (bind X (TFun (TVar Y) (TFun TUnit TUnit)) tempty) (TFun TUnit TUnit).
+        Proof. ex222 (TVar Y). Qed.
+
+        Definition term : expr := 
+            EFun x (TVar X) (EFun y (TVar Y) (EFun z (TVar Z) 
+                (EApp (EApp (EVar x) (EVar z)) (EApp (EVar y) (EVar z))))).
+
+        Example ex2231 : 
+            let s := (bind Y (TFun (TVar Z) TUnit) (bind X (TFun (TVar Z) (TFun TUnit TUnit)) tempty)) in
+            solution tempty term s (sub_type s (TFun (TVar X) (TFun (TVar Y) (TFun (TVar Z) TUnit)))).
+        Proof.
+            unfold solution. simpl.
+            repeat apply check_fun.
+            apply check_app with (t1 := TUnit).
+            - apply check_app with (t1 := TVar Z);
+                constructor; reflexivity.
+            - apply check_app with (t1 := TVar Z);
+                constructor; reflexivity.
+        Qed.
+
+        Ltac ct_app_apply :=
+            apply ct_app; 
+            try (intros HF; simpl in HF;
+                subst; discriminate);
+            try (intros HF; simpl in HF;
+                subst; contradiction).
+
+        (* MSet library is a pain to work with... *)
+        Axiom empty_inter :
+            forall (x y : id),
+            x <> y <-> 
+            IS.Empty (IS.inter (IS.singleton x) (IS.singleton y)).
+
+        Example ex2233 :
+            exists (t : type) (N : names) (C : constraint),
+            constraint_type tempty term t N C.
+        Proof.
+            unfold term.
+            remember "T" as T in *.
+            remember "U" as U in *.
+            remember "V" as V in *.
+            remember "W" as W in *.
+            exists (TFun (TVar X) (TFun (TVar Y) (TFun (TVar Z) (TVar W)))).
+            exists (IS.add W 
+                (IS.union 
+                    (IS.add U (IS.union IS.empty IS.empty))
+                    (IS.add V (IS.union IS.empty IS.empty)))).
+            exists ((TVar U, TFun (TVar V) (TVar W)) :: 
+                ((TVar X, TFun (TVar Z) (TVar U)) :: [] ++ []) ++
+                ((TVar Y, TFun (TVar Z) (TVar V)) :: [] ++ [])).
+            repeat apply ct_fun.
+            ct_app_apply.
+            - ct_app_apply;
+                try (constructor; reflexivity);
+                try apply ISP.empty_inter_1;
+                try apply ISP.empty_inter_2;
+                try apply IS.empty_spec.
+                + intros HF; inv HF.
+                + intros HF; inv HF.
+                + intros q Q Hq HIn.
+                    destruct (IdDec.eq_dec z q) as [Hqz | Hqz];
+                    destruct (IdDec.eq_dec y q) as [Hqy | Hqy];
+                    destruct (IdDec.eq_dec x q) as [Hqx | Hqx];
+                    try rewrite Hqz in *; 
+                    try rewrite Hqy in *;
+                    try rewrite Hqx in *;
+                    try (rewrite <- (bind_complete q z Q (TVar Z) Hqz) in Hq);
+                    try (rewrite <- (bind_complete q y Q (TVar Y) Hqy) in Hq);
+                    try (rewrite bind_correct in Hq;
+                        injintrosubst Hq; simpl in HIn;
+                        discriminate).
+                    unfold bind in Hq.
+                    apply eqb_neq in Hqx. rewrite Hqx in Hq.
+                    unfold tempty in Hq. discriminate.
+            - ct_app_apply;
+                try (constructor; reflexivity);
+                try apply ISP.empty_inter_1;
+                try apply ISP.empty_inter_2;
+                try apply IS.empty_spec.
+                + intros HF; inv HF.
+                + intros HF; inv HF.
+                + intros q Q Hq HIn.
+                    destruct (IdDec.eq_dec z q) as [Hqz | Hqz];
+                    destruct (IdDec.eq_dec y q) as [Hqy | Hqy];
+                    destruct (IdDec.eq_dec x q) as [Hqx | Hqx];
+                    try rewrite Hqz in *; 
+                    try rewrite Hqy in *;
+                    try rewrite Hqx in *;
+                    try (rewrite <- (bind_complete q z Q (TVar Z) Hqz) in Hq);
+                    try (rewrite <- (bind_complete q y Q (TVar Y) Hqy) in Hq);
+                    try (rewrite bind_correct in Hq;
+                        injintrosubst Hq; simpl in HIn;
+                        discriminate).
+                    unfold bind in Hq.
+                    apply eqb_neq in Hqx. rewrite Hqx in Hq.
+                    unfold tempty in Hq. discriminate.
+            - rewrite ISP.empty_union_1; auto.
+                rewrite <- ISP.singleton_equal_add.
+                rewrite <- ISP.singleton_equal_add.
+                apply empty_inter. intros HVU.
+                subst. discriminate.
+            - rewrite ISP.empty_union_1; auto.
+                rewrite <- ISP.singleton_equal_add. simpl.
+                apply empty_inter. intros HVU.
+                subst. discriminate.
+            - rewrite ISP.empty_union_1; auto.
+                rewrite <- ISP.singleton_equal_add. simpl.
+                apply empty_inter. intros HVU.
+                subst. discriminate.
+            - intros HF.
+                rewrite ISP.empty_union_1 in HF; auto.
+                rewrite <- ISP.singleton_equal_add in HF.
+                inv HF; try discriminate. inv H0.
+            - intros HF.
+                rewrite ISP.empty_union_1 in HF; auto.
+                rewrite <- ISP.singleton_equal_add in HF.
+                inv HF; try discriminate. inv H0.
+            - intros HF. simpl in HF. 
+                destruct HF as [HF | HF]; contradiction.
+            - intros HF. simpl in HF. 
+                destruct HF as [HF | HF]; contradiction.
+            - intros HF. simpl in HF. inv HF.
+                + destruct H0 as [HX | [HZ | HU]];
+                    discriminate.
+                + inv H0.
+            - intros HF. simpl in HF. inv HF.
+                + destruct H0 as [HX | [HZ | HU]];
+                    discriminate.
+                + inv H0.
+            - intros q Q Hq HIn.
                 destruct (IdDec.eq_dec z q) as [Hqz | Hqz];
                 destruct (IdDec.eq_dec y q) as [Hqy | Hqy];
                 destruct (IdDec.eq_dec x q) as [Hqx | Hqx];
@@ -750,76 +785,17 @@ Section Examples.
                     discriminate).
                 unfold bind in Hq.
                 apply eqb_neq in Hqx. rewrite Hqx in Hq.
-                unfold empty in Hq. discriminate.
-        - ct_app_apply;
-            try (constructor; reflexivity);
-            try apply ISP.empty_inter_1;
-            try apply ISP.empty_inter_2;
-            try apply IS.empty_spec.
-            + intros HF; inv HF.
-            + intros HF; inv HF.
-            + intros q Q Hq HIn.
-                destruct (IdDec.eq_dec z q) as [Hqz | Hqz];
-                destruct (IdDec.eq_dec y q) as [Hqy | Hqy];
-                destruct (IdDec.eq_dec x q) as [Hqx | Hqx];
-                try rewrite Hqz in *; 
-                try rewrite Hqy in *;
-                try rewrite Hqx in *;
-                try (rewrite <- (bind_complete q z Q (TVar Z) Hqz) in Hq);
-                try (rewrite <- (bind_complete q y Q (TVar Y) Hqy) in Hq);
-                try (rewrite bind_correct in Hq;
-                    injintrosubst Hq; simpl in HIn;
-                    discriminate).
-                unfold bind in Hq.
-                apply eqb_neq in Hqx. rewrite Hqx in Hq.
-                unfold empty in Hq. discriminate.
-        - rewrite ISP.empty_union_1; auto.
-            rewrite <- ISP.singleton_equal_add.
-            rewrite <- ISP.singleton_equal_add.
-            apply empty_inter. intros HVU.
-            subst. discriminate.
-        - rewrite ISP.empty_union_1; auto.
-            rewrite <- ISP.singleton_equal_add. simpl.
-            apply empty_inter. intros HVU.
-            subst. discriminate.
-        - rewrite ISP.empty_union_1; auto.
-            rewrite <- ISP.singleton_equal_add. simpl.
-            apply empty_inter. intros HVU.
-            subst. discriminate.
-        - intros HF.
-            rewrite ISP.empty_union_1 in HF; auto.
-            rewrite <- ISP.singleton_equal_add in HF.
-            inv HF; try discriminate. inv H0.
-        - intros HF.
-            rewrite ISP.empty_union_1 in HF; auto.
-            rewrite <- ISP.singleton_equal_add in HF.
-            inv HF; try discriminate. inv H0.
-        - intros HF. simpl in HF. 
-            destruct HF as [HF | HF]; contradiction.
-        - intros HF. simpl in HF. 
-            destruct HF as [HF | HF]; contradiction.
-        - intros HF. simpl in HF. inv HF.
-            + destruct H0 as [HX | [HZ | HU]];
-                discriminate.
-            + inv H0.
-        - intros HF. simpl in HF. inv HF.
-            + destruct H0 as [HX | [HZ | HU]];
-                discriminate.
-            + inv H0.
-        - intros q Q Hq HIn.
-            destruct (IdDec.eq_dec z q) as [Hqz | Hqz];
-            destruct (IdDec.eq_dec y q) as [Hqy | Hqy];
-            destruct (IdDec.eq_dec x q) as [Hqx | Hqx];
-            try rewrite Hqz in *; 
-            try rewrite Hqy in *;
-            try rewrite Hqx in *;
-            try (rewrite <- (bind_complete q z Q (TVar Z) Hqz) in Hq);
-            try (rewrite <- (bind_complete q y Q (TVar Y) Hqy) in Hq);
-            try (rewrite bind_correct in Hq;
-                injintrosubst Hq; simpl in HIn;
-                discriminate).
-            unfold bind in Hq.
-            apply eqb_neq in Hqx. rewrite Hqx in Hq.
-            unfold empty in Hq. discriminate.
-    Qed.
-End Examples.
+                unfold tempty in Hq. discriminate.
+        Qed.
+    End Examples.
+End Monomorphic.
+
+Module Polymorphic.
+    Module M := Monomorphic.
+
+    Definition type : Type := M.type.
+
+    Inductive poly : Type :=
+        | PType (t : type)
+        | PForall (X : id) (t : poly).
+End Polymorphic.
